theories/typing/uniq_array_util.v
@@ -6,10 +6,10 @@ Implicit Type 𝔄 𝔅: syn_type.
 Section uniq_array_util.
   Context `{!typeG Σ}.
 
-  Lemma ty_share_big_sepL_uniq_own {𝔄} (ty: type 𝔄) n (vπξil: vec _ n)
+  Lemma ty_share_big_sepL_uniq_body {𝔄} (ty: type 𝔄) n (vπξil: vec _ n)
       d κ tid l κ' q E :
     ↑lftN ⊆ E → lft_ctx -∗ κ' ⊑ κ -∗ κ' ⊑ ty.(ty_lft) -∗
-    &{κ'} ([∗ list] i ↦ vπξi ∈ vπξil, uniq_own ty vπξi.1 vπξi.2 d κ tid (l +ₗ[ty] i)) -∗
+    &{κ'} ([∗ list] i ↦ vπξi ∈ vπξil, uniq_body ty vπξi.1 vπξi.2 d κ tid (l +ₗ[ty] i)) -∗
     q.[κ'] ={E}=∗ |={E}▷=>^(S d) |={E}=>
       let ξl := vmap (λ vπξi, PrVar (𝔄 ↾ prval_to_inh vπξi.1) vπξi.2) vπξil in
       &{κ'} 1:+[ξl] ∗
@@ -22,29 +22,29 @@ Section uniq_array_util.
     { iApply step_fupdN_full_intro. iFrame "κ'".
       by iMod (bor_create _ _ True%I with "LFT [//]") as "[$ _]". }
     iDestruct "Bors" as "[Bor Bors]". iDestruct "κ'" as "[κ' κ'₊]".
-    iMod (ty_share_uniq_own with "LFT In In' Bor κ'") as "Upd"; [done|].
+    iMod (ty_share_uniq_body with "LFT In In' Bor κ'") as "Upd"; [done|].
     setoid_rewrite <-shift_loc_assoc_nat. iMod ("IH" with "κ'₊ Bors") as "Upd'".
     iCombine "Upd Upd'" as "Upd". iApply (step_fupdN_wand _ _ (S _) with "Upd").
     iIntros "!> [>(ξ &$&$) >(ξl &$&$)]".
     by iMod (bor_combine with "LFT ξ ξl") as "$".
   Qed.
 
-  Lemma ty_own_proph_big_sepL_uniq_own {𝔄} (ty: type 𝔄) n (vπξil: vec _ n)
+  Lemma ty_own_proph_big_sepL_uniq_body {𝔄} (ty: type 𝔄) n (vπξil: vec _ n)
       d κ tid l κ' q E :
     ↑lftN ⊆ E → lft_ctx -∗ κ' ⊑ κ -∗ κ' ⊑ ty.(ty_lft) -∗
-    ([∗ list] i ↦ vπξi ∈ vπξil, uniq_own ty vπξi.1 vπξi.2 d κ tid (l +ₗ[ty] i)) -∗
+    ([∗ list] i ↦ vπξi ∈ vπξil, uniq_body ty vπξi.1 vπξi.2 d κ tid (l +ₗ[ty] i)) -∗
     q.[κ'] ={E}=∗ |={E}▷=>^(S d) |={E}=>
       let ξl := vmap (λ vπξi, PrVar (𝔄 ↾ prval_to_inh vπξi.1) vπξi.2) vπξil in
       ∃ζl q', ⌜vapply (vmap fst vπξil) ./ ζl⌝ ∗ q':+[ζl ++ ξl] ∗
         (q':+[ζl ++ ξl] ={E}=∗
-          ([∗ list] i ↦ vπξi ∈ vπξil, uniq_own ty vπξi.1 vπξi.2 d κ tid (l +ₗ[ty] i)) ∗
+          ([∗ list] i ↦ vπξi ∈ vπξil, uniq_body ty vπξi.1 vπξi.2 d κ tid (l +ₗ[ty] i)) ∗
           q.[κ']).
   Proof.
     iIntros (?) "#LFT #In #In' uniqs κ'". iInduction vπξil as [|] "IH" forall (q l).
     { iApply step_fupdN_full_intro. iIntros "!>!>". iExists [], 1%Qp.
       do 2 (iSplit; [done|]). iIntros. by iFrame. }
     iDestruct "uniqs" as "[uniq uniqs]". iDestruct "κ'" as "[κ' κ'₊]"=>/=.
-    iMod (ty_own_proph_uniq_own with "LFT In In' uniq κ'") as "Upd"; [done|].
+    iMod (ty_own_proph_uniq_body with "LFT In In' uniq κ'") as "Upd"; [done|].
     setoid_rewrite <-shift_loc_assoc_nat. iMod ("IH" with "uniqs κ'₊") as "Upd'".
     iCombine "Upd Upd'" as "Upd". iApply (step_fupdN_wand _ _ (S _) with "Upd").
     iIntros "!> [>(%&%&%& [ζl ξ] & Touniq) >(%&%&%& [ζl' ξl] & Touniqs)] !>".
@@ -59,10 +59,10 @@ Section uniq_array_util.
     by iMod ("Touniqs" with "[$ζl' $ξl]") as "[$$]".
   Qed.
 
-  Lemma resolve_big_sepL_uniq_own {𝔄} (ty: type 𝔄) n (vπξil: vec _ n) d κ tid l E L q F :
+  Lemma resolve_big_sepL_uniq_body {𝔄} (ty: type 𝔄) n (vπξil: vec _ n) d κ tid l E L q F :
     lctx_lft_alive E L κ → ↑lftN ∪ ↑prophN ⊆ F →
     lft_ctx -∗ proph_ctx -∗ κ ⊑ ty.(ty_lft) -∗ elctx_interp E -∗ llctx_interp L q -∗
-    ([∗ list] i ↦ vπξi ∈ vπξil, uniq_own ty vπξi.1 vπξi.2 d κ tid (l +ₗ[ty] i))
+    ([∗ list] i ↦ vπξi ∈ vπξil, uniq_body ty vπξi.1 vπξi.2 d κ tid (l +ₗ[ty] i))
       ={F}=∗ |={F}▷=>^(S d) |={F}=>
       let φπ π := lforall (λ vπξi,
         let ξ := PrVar (𝔄 ↾ prval_to_inh vπξi.1) vπξi.2 in π ξ = vπξi.1 π) vπξil in
@@ -71,40 +71,40 @@ Section uniq_array_util.
     iIntros (??) "#LFT #PROPH #In #E L uniqs". iInduction vπξil as [|] "IH" forall (q l).
     { iApply step_fupdN_full_intro. iFrame "L". by iApply proph_obs_true. }
     iDestruct "uniqs" as "[uniq uniqs]". iDestruct "L" as "[L L₊]"=>/=.
-    iMod (resolve_uniq_own with "LFT PROPH In E L uniq") as "Upd"; [done..|].
+    iMod (resolve_uniq_body with "LFT PROPH In E L uniq") as "Upd"; [done..|].
     setoid_rewrite <-shift_loc_assoc_nat. iMod ("IH" with "L₊ uniqs") as "Upd'".
     iCombine "Upd Upd'" as "Upd". iApply (step_fupdN_wand _ _ (S _) with "Upd").
     iIntros "!> [>[Obs $] >[Obs' $]]". by iCombine "Obs Obs'" as "$".
   Qed.
 
-  Lemma real_big_sepL_uniq_own {𝔄 𝔅} (ty: type 𝔄) n (vπξil: vec _ n)
+  Lemma real_big_sepL_uniq_body {𝔄 𝔅} (ty: type 𝔄) n (vπξil: vec _ n)
       d κ tid l E L (f: _ → 𝔅) q F :
     lctx_lft_alive E L κ → real E L ty f → ↑lftN ⊆ F →
     lft_ctx -∗ elctx_interp E -∗ llctx_interp L q -∗
-    ([∗ list] i ↦ vπξi ∈ vπξil, uniq_own ty vπξi.1 vπξi.2 d κ tid (l +ₗ[ty] i))
+    ([∗ list] i ↦ vπξi ∈ vπξil, uniq_body ty vπξi.1 vπξi.2 d κ tid (l +ₗ[ty] i))
       ={F}=∗ |={F}▷=>^(S d) |={F}=>
       ⌜∃v, vapply (vmap ((f ∘.) ∘ fst) vπξil) = const v⌝ ∗ llctx_interp L q ∗
-      ([∗ list] i ↦ vπξi ∈ vπξil, uniq_own ty vπξi.1 vπξi.2 d κ tid (l +ₗ[ty] i)).
+      ([∗ list] i ↦ vπξi ∈ vπξil, uniq_body ty vπξi.1 vπξi.2 d κ tid (l +ₗ[ty] i)).
   Proof.
     iIntros (???) "#LFT #E L uniqs". iInduction vπξil as [|] "IH" forall (q l).
     { iApply step_fupdN_full_intro. iIntros "!>!>". iFrame "L".
       iSplit; [|done]. by iExists [#]. }
     iDestruct "uniqs" as "[uniq uniqs]". iDestruct "L" as "[L L₊]"=>/=.
-    iMod (real_uniq_own with "LFT E L uniq") as "Upd"; [done..|].
+    iMod (real_uniq_body with "LFT E L uniq") as "Upd"; [done..|].
     setoid_rewrite <-shift_loc_assoc_nat. iMod ("IH" with "L₊ uniqs") as "Upd'".
     iCombine "Upd Upd'" as "Upd". iApply (step_fupdN_wand _ _ (S _) with "Upd").
     iIntros "!> [>([%v ->]&$&$) >([%vl %Eq]&$&$)] !%". exists (v ::: vl).
     fun_ext=>/= ?. by rewrite Eq.
   Qed.
 
-  Lemma incl_big_sepL_uniq_own {𝔄} (ty ty': type 𝔄) vπξil d κ κ' tid l :
+  Lemma incl_big_sepL_uniq_body {𝔄} (ty ty': type 𝔄) vπξil d κ κ' tid l :
     κ' ⊑ κ -∗ □ (∀vπ d tid vl, ty.(ty_own) vπ d tid vl ↔ ty'.(ty_own) vπ d tid vl) -∗
-    ([∗ list] i ↦ vπξi ∈ vπξil, uniq_own ty vπξi.1 vπξi.2 d κ tid (l +ₗ[ty] i)) -∗
-    [∗ list] i ↦ vπξi ∈ vπξil, uniq_own ty' vπξi.1 vπξi.2 d κ' tid (l +ₗ[ty] i).
+    ([∗ list] i ↦ vπξi ∈ vπξil, uniq_body ty vπξi.1 vπξi.2 d κ tid (l +ₗ[ty] i)) -∗
+    [∗ list] i ↦ vπξi ∈ vπξil, uniq_body ty' vπξi.1 vπξi.2 d κ' tid (l +ₗ[ty] i).
   Proof.
     iIntros "#InLft #EqOwn uniqs". iInduction vπξil as [|] "IH" forall (l); [done|].
     iDestruct "uniqs" as "[uniq uniqs]".
-    iDestruct (incl_uniq_own with "InLft EqOwn uniq") as "$"=>/=.
+    iDestruct (incl_uniq_body with "InLft EqOwn uniq") as "$"=>/=.
     setoid_rewrite <-shift_loc_assoc_nat. iDestruct ("IH" with "uniqs") as "$".
   Qed.
 
